STLC_SuccNat/Lifted_Norm.v
@@ -1,7 +1,7 @@
 Require Import String List Maps.
 Import ListNotations.
 Require Import STLC_SuccNat.
-Require Import Lifted_STLC_SuccNat.
+Require Import Presence_Conditions Lifted_STLC_SuccNat.
 Require Import Environments.
 
 Hint Constructors multi : core.
@@ -32,7 +32,9 @@ Inductive appears_free_in' : string -> tm' -> Prop :=
     y <> x -> appears_free_in' x t12' ->
       appears_free_in' x (abs' y T11' t12')
   (* nats*)
-  |afi_succ' : forall x t1', appears_free_in' x t1' -> appears_free_in' x (succ' t1').
+  |afi_succ' : forall x t1', appears_free_in' x t1' -> appears_free_in' x (succ' t1')
+  |afi_add1' : forall x t1' t2', appears_free_in' x t1' -> appears_free_in' x (add' t1' t2')
+  |afi_add2' : forall x t1' t2', appears_free_in' x t2' -> appears_free_in' x (add' t1' t2').
 
 Hint Constructors appears_free_in' : core.
 
@@ -200,8 +202,13 @@ Proof with eauto.
     reflexivity.
     intros H; eauto.
     intros H; eauto.
-   - (* Succ' *)
+ - (* Succ' *)
     rewrite IHt'...
+ - (* Add' *)
+    rewrite IHt'1, IHt'2.
+    reflexivity.
+    intros H; eauto.
+    intros H; eauto.
 Qed.
 
 Lemma subst'_closed': forall t',
@@ -241,6 +248,8 @@ Proof with eauto.  (* rather slow this way *)
      inversion A.
     - (* succ' *)
      inversion A; subst...
+    - (* add' *)
+     inversion A; subst...
 Qed.
 
 Lemma duplicate_subst' : forall t1' x t' v',
@@ -274,6 +283,8 @@ Proof with eauto.
    reflexivity.
   - (* succ' *)
    rewrite IHt'...
+  - (* add' *)
+   rewrite IHt'1, IHt'2...
 Qed.
 
 Lemma subst'_msubst': forall env' x v' t', closed' v' -> closed'_env' env' ->
@@ -408,7 +419,7 @@ Proof.
          apply multistep'_preserves_R1' with (msubst' ((x,v)::env0') t').
             eapply T_App'. eauto.
             apply R'_typable_empty; auto.
-            eapply multi_step'_trans. eapply multistep'_App2'; eauto.
+            eapply multi_step'_trans. eapply multistep'_app2'; eauto.
             eapply multi_step with (y:= (msubst' ((x, v) :: env0') t')); [|apply multi_refl].
             simpl.  rewrite subst'_msubst'.
             eapply ST_AppAbs'; eauto.
@@ -440,6 +451,29 @@ Proof.
       eauto.
       apply (canonical_forms_nat' v A) in Hv as [n Hv].
       rewrite Hv. exists (const' (map (fun '(n0,pc) => (S (n0),pc)) n)); eauto.
+      auto.
+  - (* T_Add' *)
+    rewrite msubst'_add'.
+    apply (IHHT1 c H env0') in V as IH1.
+    apply (IHHT2 c H env0') in V as IH2.
+    clear IHHT1 IHHT2.
+    destruct (R'_halts' IH1) as [v1' [Hm1' Hv1']].
+    destruct (R'_halts' IH2) as [v2' [Hm2' Hv2']].
+    eapply multistep'_preserves_R1'.
+      eauto using R'_typable_empty.
+      eapply multi_step'_trans.
+      eapply multistep'_add1'. exact Hm1'.
+      eapply multistep'_add2'; eassumption.
+    eapply (multistep'_preserves_R' _ _ _ Hm1') in IH1
+      as [A1 [B1 _]].
+    eapply (multistep'_preserves_R' _ _ _ Hm2') in IH2
+      as [A2 [B2 _]].
+    split; [|split].
+      eauto.
+      apply (canonical_forms_nat' v1' A1) in Hv1' as [n1' Hv1'].
+      apply (canonical_forms_nat' v2' A2) in Hv2' as [n2' Hv2'].
+      rewrite Hv1', Hv2'. exists (const' (app_binop Nat.add n1' n2')).
+      split. econstructor. apply ST_AddConst'. apply multi_refl. auto.
       auto.
 Qed.
 
